Began dense formulation

LogicalRefinement/Denot/Basic.lean
@@ -10,7 +10,6 @@ open Annot
 -- TODO: report spurious unused variable warning...
 def Term.denote_ty (A: Term) 
   {Γ: Stlc.Context}
-  (σ: Sparsity)
   (G: Γ.interp)
   (a: A.stlc_ty.interp): Prop
   := match A with
@@ -22,60 +21,56 @@ def Term.denote_ty (A: Term)
     match a with
     | some a =>
       ∀x: A.stlc_ty.interp,
-        A.denote_ty σ G x ->
-        @denote_ty B (A.stlc_ty::Γ) (true::σ) (x, G) (x.bind_val a)
+        A.denote_ty G x ->
+        @denote_ty B (A.stlc_ty::Γ) (x, G) (x.bind_val a)
     | none => False
   | abs TermKind.sigma A B => 
     match a with
     | some (a, b) => 
       let a := Ty.eager a;
       let b := Ty.eager b;
-      A.denote_ty σ G a ∧ @denote_ty B (A.stlc_ty::Γ) (true::σ) (a, G) b
+      A.denote_ty G a ∧ @denote_ty B (A.stlc_ty::Γ) (a, G) b
     | none => False
   | bin TermKind.coprod A B =>
     match a with
     | some a => 
       match a with
-      | Sum.inl a => A.denote_ty σ G (Ty.eager a)
-      | Sum.inr b => B.denote_ty σ G (Ty.eager b)
+      | Sum.inl a => A.denote_ty G (Ty.eager a)
+      | Sum.inr b => B.denote_ty G (Ty.eager b)
     | none => False
-  | abs TermKind.assume φ A => 
-    a ≠ none ∧
-    ((φ.denote_ty σ G none) -> (A.denote_ty (false::σ) G a))
+  | abs TermKind.assume φ A => (φ.denote_ty G none) -> (A.denote_ty G sorry)
   | abs TermKind.set A φ => 
-    A.denote_ty σ G a ∧ @denote_ty φ (A.stlc_ty::Γ) (true::σ) (a, G) none
-  | abs TermKind.intersect A B => 
-    a ≠ none ∧
+    A.denote_ty G a ∧ @denote_ty φ (A.stlc_ty::Γ) (a, G) none
+  | abs TermKind.intersect A B =>
     ∀x: A.stlc_ty.interp,
-      A.denote_ty σ G x ->
-      @denote_ty B (A.stlc_ty::Γ) (true::σ) (x, G) a
+      A.denote_ty G x ->
+      @denote_ty B (A.stlc_ty::Γ) (x, G) sorry
   | abs TermKind.union A B => 
-    a ≠ none ∧
     ∃x: A.stlc_ty.interp,
-      A.denote_ty σ G x ∧
-      @denote_ty B (A.stlc_ty::Γ) (true::σ) (x, G) a
+      A.denote_ty G x ∧
+      @denote_ty B (A.stlc_ty::Γ) (x, G) a
   | const TermKind.top => True
   | const TermKind.bot => False
   | abs TermKind.dimplies A B => 
     --TODO: think about this...
-    (A.denote_ty σ G none) -> (B.denote_ty (false::σ) G none)
+    (A.denote_ty G none) -> (B.denote_ty G none)
   | abs TermKind.dand A B =>
     --TODO: think about this...
-    A.denote_ty σ G none ∧ B.denote_ty (false::σ) G none
+    A.denote_ty G none ∧ B.denote_ty G none
   | bin TermKind.or A B => 
-    A.denote_ty σ G none ∨ B.denote_ty σ G none
+    A.denote_ty G none ∨ B.denote_ty G none
   | abs TermKind.forall_ A φ => 
     ∀x: A.stlc_ty.interp,
-      A.denote_ty σ G x ->
-      @denote_ty φ (A.stlc_ty::Γ) (true::σ) (x, G) none
+      A.denote_ty G x ->
+      @denote_ty φ (A.stlc_ty::Γ) (x, G) none
   | abs TermKind.exists_ A φ => 
     ∃x: A.stlc_ty.interp,
-      A.denote_ty σ G x ∧
-      @denote_ty φ (A.stlc_ty::Γ) (true::σ) (x, G) none
+      A.denote_ty G x ∧
+      @denote_ty φ (A.stlc_ty::Γ) (x, G) none
   | tri TermKind.eq A x y => 
     --TODO: this should probably be a forall; makes life a little easier...
-    ∃ px: Γ ⊧ x.stlc σ: A.stlc_ty, 
-    ∃ py: Γ ⊧ y.stlc σ: A.stlc_ty,
+    ∃ px: Γ ⊧ x.stlc: A.stlc_ty, 
+    ∃ py: Γ ⊧ y.stlc: A.stlc_ty,
     px.interp G = py.interp G
   | const TermKind.nats => 
     match a with
@@ -85,18 +80,8 @@ def Term.denote_ty (A: Term)
 
 abbrev Term.denote_prop (A: Term) 
   {Γ: Stlc.Context}
-  (σ: Sparsity)
   (G: Γ.interp): Prop
-  := A.denote_ty σ G none
-
-abbrev Term.denote_ty' (A: Term) {Γ: Context}
-  (G: Γ.upgrade.stlc.interp)
-  (a: A.stlc_ty.interp): Prop
-  := A.denote_ty Γ.upgrade.sparsity G a
-
-abbrev Term.denote_prop' (A: Term) {Γ: Context}
-  (G: Γ.upgrade.stlc.interp): Prop
-  := A.denote_prop Γ.upgrade.sparsity G
+  := A.denote_ty G none
 
 notation G "⊧" a "↓" σ "∈" A => Term.denote_ty A σ G a
 notation G "⊧" a "∈" A => Term.denote_ty' A G a
@@ -108,7 +93,7 @@ theorem Term.denote_ty_transport
   (HΓ: Γ = Γ')
   (HG: G = HΓ ▸ G')
   (Ha: a' = HA ▸ a)
-  : @denote_ty' A Γ G a -> @denote_ty' A' Γ' G' a'
+  : @denote_ty A Γ G a -> @denote_ty A' Γ' G' a'
   := by {
     cases HA;
     cases HΓ;
@@ -118,9 +103,9 @@ theorem Term.denote_ty_transport
   }
 
 theorem HasType.denote_ty_non_null 
-  {Γ} {Δ: Stlc.Context} {G: Δ.interp} {A σ}:
+  {Γ} {Δ: Stlc.Context} {G: Δ.interp} {A}:
   (Γ ⊢ A: type) ->
-  ¬(A.denote_ty σ G none)
+  ¬(A.denote_ty G none)
   := by {
     generalize HS: sort type = S;
     intro HA;
@@ -129,22 +114,16 @@ theorem HasType.denote_ty_non_null
       dsimp only [Term.denote_ty]
       intro ⟨HA, _⟩;
       exact IA rfl HA
-    | assume => 
-      intro ⟨H, _⟩;
-      exact H rfl
-    | intersect => 
-      intro ⟨H, _⟩;
-      exact H rfl
-    | union => 
-      intro ⟨H, _⟩;
-      exact H rfl
+    | assume => sorry
+    | intersect => sorry
+    | union => sorry
     | _ => cases HS <;> intro H <;> cases H
   }
 
 --TODO: report spurious unused variable warning
 theorem HasType.denote_ty_some {Δ: Stlc.Context} {G: Δ.interp}
   (H: Γ ⊢ A: type)
-  (D: A.denote_ty σ G a)
+  (D: A.denote_ty G a)
   : ∃a': A.stlc_ty.interp_val, a = some a'
   := match a with
     | some a => ⟨a, rfl⟩
@@ -157,28 +136,19 @@ abbrev Annot.denote (A: Annot) {Γ: Stlc.Context}
   (a: A.stlc_ty.interp): Prop
   := match A with
   | sort _ => True
-  | expr type A => A.denote_ty σ G a
-  | expr prop A => A.denote_ty σ G none
+  | expr type A => A.denote_ty G a
+  | expr prop A => A.denote_ty G none
 
-abbrev Annot.denote' (A: Annot) (Γ: Context)
-  (G: Γ.upgrade.stlc.interp)
-  (a: A.stlc_ty.interp): Prop
-  := match A with
-  | sort s => True
-  | expr type A => A.denote_ty' G a
-  | expr prop A => A.denote_ty' G none
-
-notation G "⊧" a "↓" σ "∈:" A => Annot.denote A σ G a
-notation G "⊧" a "∈:" A => Annot.denote' A G a
+notation G "⊧" a "∈" A => Annot.denote A G a
 
 def Context.denote: (Γ: Context) -> Γ.upgrade.stlc.interp -> Prop
 | [], () => True
 | (Hyp.mk A (HypKind.val type))::Γ, (a, G) => 
-  A.denote_ty (upgrade Γ).sparsity G a ∧ denote Γ G
-| (Hyp.mk φ (HypKind.val prop))::Γ, G =>
-  φ.denote_ty (upgrade Γ).sparsity G none ∧ denote Γ G
+  A.denote_ty G a ∧ denote Γ G
+| (Hyp.mk φ (HypKind.val prop))::Γ, (a, G) =>
+  φ.denote_ty G none ∧ denote Γ sorry
 | (Hyp.mk A HypKind.gst)::Γ, (a, G) =>
-  A.denote_ty (upgrade Γ).sparsity G a ∧ denote Γ G
+  A.denote_ty G a ∧ denote Γ G
 
 theorem Context.denote.upgrade_helper {Γ: Context}
   : Γ.denote = Context.upgrade_idem.symm ▸ Γ.upgrade.denote
