LogicalRefinement/Stlc/Interp.lean
@@ -11,30 +11,28 @@ def Term.stlc_ty: Term -> Ty
 | abs TermKind.pi A B => Ty.arrow A.stlc_ty B.stlc_ty
 | abs TermKind.sigma A B => Ty.prod A.stlc_ty B.stlc_ty
 | bin TermKind.coprod A B => Ty.coprod A.stlc_ty B.stlc_ty
-| abs TermKind.assume _ A => A.stlc_ty
+| abs TermKind.assume _ A => Ty.arrow Ty.unit A.stlc_ty
 | abs TermKind.set A _ => A.stlc_ty
-| abs TermKind.intersect _ B => B.stlc_ty
+| abs TermKind.intersect _ B => Ty.arrow Ty.unit B.stlc_ty
 | abs TermKind.union _ B => B.stlc_ty
 | const TermKind.nats => Ty.nats
-| _ => Ty.bot
+| _ => Ty.unit
 
-theorem HasType.prop_is_bot {Γ A}: (Γ ⊢ A: prop) -> A.stlc_ty = Ty.bot
+theorem HasType.prop_is_unit {Γ A}: (Γ ⊢ A: prop) -> A.stlc_ty = Ty.unit
 := by {
   intro H;
   cases H <;> rfl
 }
 
 def Annot.stlc_ty: Annot -> Ty
-| expr type A => A.stlc_ty
-| _ => Ty.bot
+| expr _ A => A.stlc_ty
+| _ => Ty.unit
 
-theorem Annot.prop_is_bot {Γ A s}: 
-  (Γ ⊢ A: prop) -> (expr s A).stlc_ty = Ty.bot
+theorem Annot.prop_is_unit {Γ A s}: 
+  (Γ ⊢ A: prop) -> (expr s A).stlc_ty = Ty.unit
   := by {
     intro H;
-    cases s with
-    | type => exact H.prop_is_bot
-    | prop => rfl
+    exact H.prop_is_unit
   }
 
 theorem Annot.sort_case {Γ A s} (H: Γ ⊢ A: sort s): 
@@ -42,163 +40,45 @@ theorem Annot.sort_case {Γ A s} (H: Γ ⊢ A: sort s):
   := by {
     cases s with
     | type => simp only [stlc_ty]
-    | prop => rw [Annot.prop_is_bot H, HasType.prop_is_bot H]
+    | prop => rw [Annot.prop_is_unit H, HasType.prop_is_unit H]
   }
 
 def Context.stlc: Context -> Stlc.Context
 | [] => []
-| (Hyp.mk A (HypKind.val type))::Hs => A.stlc_ty::(stlc Hs)
-| _::Hs => stlc Hs
+| (Hyp.mk A (HypKind.val _))::Hs => A.stlc_ty::(stlc Hs)
+| (Hyp.mk _ HypKind.gst)::Hs => Ty.unit::(stlc Hs)
 
-@[simp]
-theorem Context.stlc_gst
-  : stlc ((Hyp.gst A)::Γ) = stlc Γ
-  := rfl
+def Term.stlc: Term -> Stlc
+| var n => Stlc.var n
+| const TermKind.nil => Stlc.nil
+| abs TermKind.lam A x => Stlc.lam A.stlc_ty x.stlc
+| tri TermKind.app P l r => Stlc.app P.stlc_ty l.stlc r.stlc
+| bin TermKind.pair l r => Stlc.pair l.stlc r.stlc
+| let_bin TermKind.let_pair P e e' => 
+  Stlc.let_pair P.stlc_ty e.stlc e'.stlc
+| unary (TermKind.inj i) e => Stlc.inj i e.stlc
+| cases TermKind.case P d l r => 
+  Stlc.case P.stlc_ty d.stlc l.stlc r.stlc
+| abs TermKind.lam_pr _ x => x.stlc
+| tri TermKind.app_pr _ e _ => e.stlc
+| bin TermKind.elem e _ => e.stlc
+| let_bin TermKind.let_set P e e' =>
+  Stlc.let_in P.stlc_ty e.stlc (Stlc.let_in Ty.unit Stlc.nil e'.stlc)
+| abs TermKind.lam_irrel _ x => x.stlc
+| tri TermKind.app_irrel _ l _ => l.stlc
+| bin TermKind.repr _ r => r.stlc
+| let_bin TermKind.let_repr P e e' => 
+  Stlc.let_in Ty.unit Stlc.nil (Stlc.let_in P.stlc_ty e.stlc e'.stlc)
+| const TermKind.zero => Stlc.zero
+| const TermKind.succ => Stlc.succ
+| nr (TermKind.natrec type) K n z s 
+  => Stlc.natrec K.stlc_ty n.stlc z.stlc 
+    (Stlc.let_in Ty.unit Stlc.nil 
+      (Stlc.let_in K.stlc_ty (Stlc.var 1) s.stlc))
+| unary TermKind.abort _ => Stlc.abort
+| _ => Stlc.abort
 
-def Context.ghosts: Context -> Stlc.Context
-| [] => []
-| (Hyp.mk A HypKind.gst)::Hs => A.stlc_ty::(ghosts Hs)
-| (Hyp.mk _ _)::Hs => (ghosts Hs)
-
-def Hyp.sparsity (H: Hyp): Bool := H.kind = HypKind.val type
-
-def Context.sparsity: Context -> Sparsity
-| [] => []
-| H::Hs => H.sparsity::(sparsity Hs)
-
-@[simp]
-theorem Context.sparsity_gst
-  : sparsity ((Hyp.gst A)::Γ) = false::(sparsity Γ)
-  := rfl
-
-@[simp]
-theorem Context.sparsity_ty
-  : sparsity ((Hyp.val A type)::Γ) = true::(sparsity Γ)
-  := rfl
-@[simp]
-theorem Context.sparsity_prop
-  : sparsity ((Hyp.val A prop)::Γ) = false::(sparsity Γ)
-  := rfl
-
-def Context.downgrade_sparsity: Context -> Sparsity
-| [] => []
-| (Hyp.mk _ (HypKind.val type))::Γ => true::(downgrade_sparsity Γ)
-| (Hyp.mk _ (HypKind.val prop))::Γ => downgrade_sparsity Γ
-| (Hyp.mk _ HypKind.gst)::Γ => false::(downgrade_sparsity Γ)
-
-@[simp]
-theorem Context.downgrade_sparsity_downgrade (Γ: Context)
-  : Γ.downgrade_sparsity.thin Γ.upgrade.stlc = Γ.stlc
-  := by {
-    induction Γ with
-    | nil => simp [downgrade_sparsity]
-    | cons H Γ I => 
-      cases H with
-      | mk A k =>
-        cases k with
-        | val s => cases s with 
-          | type => 
-            simp [Sparsity.thin] at *
-            rw [I]
-            rfl
-          | prop => exact I
-        | gst => exact I
-  }
-
-def Stlc.Context.interp.downgrade 
-  {Γ: _root_.Context} (G: Γ.upgrade.stlc.interp)
-  : Γ.stlc.interp
-  := by {
-    rw [<-Context.downgrade_sparsity_downgrade]
-    apply G.thin
-  }
-
-@[simp]
-theorem Stlc.Context.interp.downgrade_gst
-  {A: Term} {Γ: _root_.Context} 
-  (x: A.stlc_ty.interp) (G: Γ.upgrade.stlc.interp)
-  : @downgrade ((Hyp.gst A)::Γ) (x, G) = G.downgrade
-  := rfl
-
-@[simp]
-theorem Stlc.Context.interp.downgrade_prop
-  {A: Term} {Γ: _root_.Context} (G: Γ.upgrade.stlc.interp)
-  : @downgrade ((Hyp.val A prop)::Γ) G = G.downgrade
-  := rfl
-
-@[simp]
-theorem Stlc.Context.interp.downgrade_ty
-  {A: Term} {Γ: _root_.Context} 
-  (x: A.stlc_ty.interp) (G: Γ.upgrade.stlc.interp)
-  : @downgrade ((Hyp.val A type)::Γ) (x, G) = (x, G.downgrade)
-  := by {
-    dsimp only [downgrade, Eq.mpr]
-    rw [monorecursor]
-    dsimp only [thin]
-    rw [monorecursor]
-    rw [pair_mono_transport]
-    rw [Context.downgrade_sparsity_downgrade]
-    rfl
-    simp only [Sparsity.thin, Context.downgrade_sparsity_downgrade]
-    rfl
-  }
-  
-theorem Context.sparsity_true {Γ: Context}
-  : H.kind = HypKind.val type -> sparsity (H::Γ) = true::Γ.sparsity
-  := by {
-    intro H;
-    simp [sparsity, Hyp.sparsity, H]
-  }
-
-theorem Context.sparsity_false {Γ: Context}
-  : H.kind ≠ HypKind.val type -> sparsity (H::Γ) = false::Γ.sparsity
-  := by {
-    cases H with
-    | mk A k =>
-      intro H;
-      simp [sparsity, Hyp.sparsity]
-      cases k with
-      | val s => cases s with | type => contradiction | prop => rfl
-      | gst => rfl
-  }
-
-def Context.stlc_ix (Γ: Context): Nat -> Nat := Γ.sparsity.ix
-
-abbrev Sparsity.stlc (σ: Sparsity) (n: Nat): Stlc
-  := if σ.dep n then Stlc.var (σ.ix n) else Stlc.abort
-
-def Term.stlc: Term -> Sparsity -> Stlc
-| var n, σ => σ.stlc n
-| const TermKind.nil, _ => Stlc.nil
-| abs TermKind.lam A x, σ => Stlc.lam A.stlc_ty (x.stlc (true::σ))
-| tri TermKind.app P l r, σ => Stlc.app P.stlc_ty (l.stlc σ) (r.stlc σ)
-| bin TermKind.pair l r, σ => Stlc.pair (l.stlc σ) (r.stlc σ)
-| let_bin TermKind.let_pair P e e', σ => 
-  Stlc.let_pair P.stlc_ty (e.stlc σ) (e'.stlc (true::true::σ))
-| unary (TermKind.inj i) e, σ => Stlc.inj i (e.stlc σ)
-| cases TermKind.case P d l r, σ => 
-  Stlc.case P.stlc_ty (d.stlc σ) (l.stlc (true::σ)) (r.stlc (true::σ))
-| abs TermKind.lam_pr _ x, σ => x.stlc (false::σ)
-| tri TermKind.app_pr _ e _, σ => e.stlc σ
-| bin TermKind.elem e _, σ => e.stlc σ
-| let_bin TermKind.let_set P e e', σ =>
-  Stlc.let_in P.stlc_ty (e.stlc σ) (e'.stlc (false::true::σ))
-| abs TermKind.lam_irrel _ x, σ => x.stlc (false::σ)
-| tri TermKind.app_irrel _ l _, σ => l.stlc σ
-| bin TermKind.repr _ r, σ => r.stlc σ
-| let_bin TermKind.let_repr P e e', σ => 
-  Stlc.let_in P.stlc_ty (e.stlc σ) (e'.stlc (true::false::σ))
-| const TermKind.zero, _ => Stlc.zero
-| const TermKind.succ, _ => Stlc.succ
-| nr (TermKind.natrec k) K n z s, σ => 
-  if k = type then
-    Stlc.natrec K.stlc_ty (n.stlc σ) (z.stlc σ) (s.stlc (true::false::σ))
-  else
-    Stlc.abort
-| unary TermKind.abort _, _ => Stlc.abort
-| _, _ => Stlc.abort
-
-def Term.stlc_var: (var v).stlc σ = σ.stlc v := rfl
+theorem Term.stlc_var: (Term.var v).stlc = Stlc.var v := rfl
 
 -- theorem Context.stlc_subst_ctx {Γ: Context}
 --   : Stlc.SubstCtx Γ.stlc_subst Γ.stlc_strict Γ.stlc
@@ -252,22 +132,25 @@ theorem Term.stlc_ty_wk1 (A: Term): (A.wk1).stlc_ty = A.stlc_ty
 }
 
 theorem Annot.stlc_ty_subst {Γ A σ s k} (H: Γ ⊢ A: sort s):
-  (expr k (A.subst σ)).stlc_ty = (expr k A).stlc_ty := by {
-    cases k with
-    | type => exact H.stlc_ty_subst
-    | prop => rfl
-  }
+  (expr k (A.subst σ)).stlc_ty = (expr k A).stlc_ty := H.stlc_ty_subst
 
 theorem Annot.stlc_ty_wk {A k}: ∀{ρ},
   (expr k (A.wk ρ)).stlc_ty = (expr k A).stlc_ty := by {
-    cases k with
-    | type => apply Term.stlc_ty_wk
-    | prop => intros; rfl
+    apply A.stlc_ty_wk
   }
 
+theorem Annot.stlc_ty_subst' {Γ A σ s k} (H: Γ ⊢ A: sort s):
+  ((expr k A).subst σ).stlc_ty = (expr k A).stlc_ty := H.stlc_ty_subst
+
+theorem Annot.stlc_ty_wk' {A k}: ∀{ρ},
+  ((expr k A).wk ρ).stlc_ty = (expr k A).stlc_ty := by {
+    apply A.stlc_ty_wk
+  }
+
+
 theorem HasVar.stlc {Γ A n}: 
-  HasVar Γ n (HypKind.val type) A ->
-  Stlc.HasVar Γ.stlc (Γ.stlc_ix n) A.stlc_ty := by {
+  HasVar Γ n (HypKind.val s) A ->
+  Stlc.HasVar Γ.stlc n A.stlc_ty := by {
     revert Γ A;
     induction n with
     | zero => 
@@ -286,102 +169,49 @@ theorem HasVar.stlc {Γ A n}:
         | succ Hv =>
           simp only [Term.wk1, Term.stlc_ty_wk]
           cases H with
-          | mk B k =>
-            cases k with
-            | val s =>
-              cases s with
-              | type => exact (I Hv).succ
-              | prop => exact (I Hv)
-            | gst => exact (I Hv)
-  }
-
-theorem HasVar.sigma_get? {Γ A n s}:
-  HasVar Γ n (HypKind.val s) A ->
-  Γ.sparsity.get? n = some (decide (s = type))
-  := by {
-    revert Γ A s;
-    induction n with
-    | zero =>
-      intro Γ A s Hv;
-      cases Hv with
-      | zero Hk =>
-        cases Hk with
-        | refl =>
-          rename AnnotSort => s;
-          cases s <;> rfl
-    | succ n I =>
-      intro Γ A s Hv;
-      cases Γ <;> cases Hv
-      rw [<-I (by assumption)]
-      rfl
-  }
-
-theorem HasVar.sigma {Γ A n s}:
-  HasVar Γ n (HypKind.val s) A ->
-  Γ.sparsity.dep n = decide (s = type)
-  := by {
-    intro H;
-    rw [Sparsity.dep_get? H.sigma_get?];
-  }
-
-theorem HasVar.sigma_ty {Γ A n}:
-  HasVar Γ n (HypKind.val type) A ->
-  Γ.sparsity.dep n = true
-  := by {
-    intro H;
-    rw [H.sigma]
-    rfl
-  }
-
-theorem HasVar.sigma_prop {Γ A n}:
-  HasVar Γ n (HypKind.val prop) A ->
-  Γ.sparsity.dep n = false
-  := by {
-    intro H;
-    exact H.sigma
+          | mk B k => cases k <;> exact (I Hv).succ
   }
 
 -- But why...
 set_option maxHeartbeats 1000000
 
 theorem HasType.stlc {Γ a A}:
-  (Γ ⊢ a : A) -> Stlc.HasType Γ.stlc (a.stlc Γ.sparsity) A.stlc_ty := by {
+  (Γ ⊢ a : A) -> Stlc.HasType Γ.stlc a.stlc A.stlc_ty := by {
     intro H;
     induction H with
     | var _ Hv => 
-      rename AnnotSort => s;
-      rw [Term.stlc_var]
-      dsimp only [Sparsity.stlc]
-      rw [Hv.sigma]
-      cases s with
-      | type => exact Stlc.HasType.var Hv.stlc
-      | prop => exact Stlc.HasType.abort
+      constructor
+      exact Hv.stlc
     | natrec HC _ _ Hs IC Ie Iz Is => 
       rename AnnotSort => k;
       cases k with
       | type =>
         dsimp only [
-          Term.stlc, Term.stlc_ty
+          Term.stlc, Term.stlc_ty, Term.subst0
         ] at *;
-        simp only [
-          Term.alpha0, Term.subst0, Annot.subst0,
-          Annot.stlc_ty_subst, Annot.stlc_ty_wk,
-          Term.stlc_ty_wk, wknth,
-          term, proof
-        ] at *
-        repeat rw [Annot.stlc_ty_subst] at *
-        repeat rw [Annot.stlc_ty_wk] at *
-        constructor <;> assumption
-        repeat first
-        | assumption
-        | (
-          apply HasType.wk_sort
-          assumption
-          repeat constructor
-          assumption
-        )
+        rw [Annot.stlc_ty_subst] at *
+        apply Stlc.HasType.natrec;
+        assumption
+        assumption
+        constructor
+        constructor
+        constructor
+        constructor
+        constructor
+        constructor
+        --TODO: fix this...
+        sorry
+        assumption
+        assumption
       | prop => exact Stlc.HasType.abort
+    | lam_pr => sorry
+    | app_pr => sorry
+    | let_set => sorry
+    | lam_irrel => sorry
+    | app_irrel => sorry
+    | let_repr => sorry
     | _ =>
+      stop
       first
       | exact Stlc.HasType.abort
       | assumption
@@ -411,11 +241,11 @@ theorem HasType.stlc {Γ a A}:
       )
   }
 
-theorem HasType.stlc_prop_is_none {Γ a A G} (H: Γ ⊢ a: expr prop A)
-  : H.stlc.interp G = none
-  := by {
-    generalize Stlc.HasType.interp _ _ = x;
-    cases x with
-    | some x => cases x
-    | none => rfl
-  }
+-- theorem HasType.stlc_prop_is_none {Γ a A G} (H: Γ ⊢ a: expr prop A)
+--   : H.stlc.interp G = none
+--   := by {
+--     generalize Stlc.HasType.interp _ _ = x;
+--     cases x with
+--     | some x => cases x
+--     | none => rfl
+--   }
