LogicalRefinement/Stlc/InterpSubst.lean
@@ -2,300 +2,42 @@ import LogicalRefinement.Untyped
 import LogicalRefinement.Typed
 import LogicalRefinement.Stlc.Basic
 import LogicalRefinement.Stlc.Interp
-import LogicalRefinement.Stlc.InterpWkUtils
-import LogicalRefinement.Stlc.InterpInv
 import LogicalRefinement.Stlc.Subst
 import LogicalRefinement.Utils
 open Annot
 open AnnotSort
 
-def Subst.stlc (σ: Subst) (Γ: Sparsity) (Δ: Sparsity): Stlc.Subst := 
-  λv => (σ (Δ.ix_inv v)).stlc Γ
+def Subst.stlc (σ: Subst): Stlc.Subst := 
+  λv => (σ v).stlc
 
-theorem Subst.stlc_lift_true {σ: Subst} {Γ Δ: Sparsity}
-  : σ.lift.stlc (true::Γ) (true::Δ) = (σ.stlc Γ Δ).lift
-  := by {
-    funext v;
-    cases v with
-    | zero => rfl
-    | succ v => exact Term.stlc_wk1_true
-  }
-
-theorem Subst.stlc_lift_false {σ: Subst} {Γ: Sparsity}
-  : σ.lift.stlc (false::Γ) (false::Δ) = σ.stlc Γ Δ
-  := by {
-    funext v;
-    cases v with
-    | zero => exact Term.stlc_wk1_false
-    | succ v => exact Term.stlc_wk1_false
-  }
+theorem Subst.stlc_lift {σ: Subst} {Γ Δ: Sparsity}
+  : σ.lift.stlc = σ.stlc.lift
+  := sorry
 
 theorem SubstCtx.stlc {σ Γ Δ} (S: SubstCtx σ Γ Δ) (HΔ: IsCtx Δ)
-  : Stlc.SubstCtx (σ.stlc Γ.sparsity Δ.sparsity) Γ.stlc Δ.stlc
-  := by {
-    intro n A Hv;
-    dsimp only [Subst.stlc]
-    have ⟨A', Hv', HA', HΔA'⟩ := Hv.interp_inv HΔ;
-    rw [<-HA']
-    rw [<-Annot.stlc_ty_subst HΔA']
-    apply HasType.stlc;
-    exact S.subst_var HΔA' Hv'
-  }
+  : Stlc.SubstCtx σ.stlc Γ.stlc Δ.stlc
+  := sorry
 
 theorem Term.term_subst_stlc_commute {Γ Δ σ a} 
   (H: Δ ⊢ a: term A) 
   (S: SubstCtx σ Γ Δ)
-  : (a.subst σ).stlc Γ.sparsity 
-  = (a.stlc Δ.sparsity).subst (σ.stlc Γ.sparsity Δ.sparsity)
-  := by {
-    have loosen: ∀{l}, (
-      ∀ {A Γ Δ σ},
-      (Δ ⊢ l: term A) ->
-      SubstCtx σ Γ Δ ->
-      (l.subst σ).stlc Γ.sparsity =
-      (l.stlc Δ.sparsity).subst (σ.stlc Γ.sparsity Δ.sparsity)
-    ) -> ∀ {A Γ Δ σ},
-      (Δ ⊢ l: term A) ->
-      SubstCtx σ Γ Δ ->
-      ∀SΓ SΔ,
-      SΓ = Γ.sparsity ->
-      SΔ = Δ.sparsity ->
-      (l.subst σ).stlc SΓ =
-      (l.stlc SΔ).subst (σ.stlc SΓ SΔ) := by {
-        intros l Il A Γ Δ σ HΔ S SΓ SΔ HSΓ HSΔ;
-        rw [HSΓ, HSΔ];
-        exact Il HΔ S
-      }
-    induction a generalizing σ Γ Δ A;
-    case var v => 
-      cases H with
-      | var HA Hv => 
-        --TODO: factor out as lemma
-        rw [Term.stlc_var]
-        dsimp only [subst, Subst.stlc, Sparsity.stlc]
-        simp only [Hv.sigma, if_pos True.intro]
-        dsimp only [Stlc.subst]
-        rw [Sparsity.ix_inv_valid]
-        rw [Hv.sigma]
-        rfl
-    case const k => cases k <;> rfl
-    case unary k t I => 
-      --TODO: change to cases h?
-      cases k with
-      | inj => 
-        have ⟨B, HB⟩: ∃B, Δ ⊢ t: term B 
-          := by cases H <;> exact ⟨_, by assumption⟩;
-        dsimp only [stlc, Stlc.subst]
-        rw [I HB S]
-      | _ => rfl
-    case let_bin k C e e' IC Ie Ie' => 
-      cases H with
-      | let_pair He HA HB HC He' =>
-        rename_i A B C;
-        let Γ' := (Hyp.val (A.subst σ) type)::Γ;
-        let Δ' := (Hyp.val A type)::Δ;
-        have S': SubstCtx σ.lift Γ' Δ'
-          := S.lift_delta (by exact HA)
-        let Γ'' := (Hyp.val (B.subst σ.lift) type)::Γ';
-        let Δ'' := (Hyp.val B type)::Δ';
-        have S'': SubstCtx σ.lift.lift Γ'' Δ''
-          := S'.lift_delta (by exact HB);
-        have Ie'' := 
-          loosen Ie' He' S'' 
-          (true::true::Γ.sparsity) (true::true::Δ.sparsity);
-        dsimp only [stlc, Stlc.subst, Subst.liftn]
-        conv =>
-          lhs
-          congr
-          . rw [(HasType.sigma HA HB).stlc_ty_subst]
-          . rw [Ie He S]
-          . rw [Ie'']
-            rw [Subst.stlc_lift_true]
-            rw [Subst.stlc_lift_true]
-      | let_set He HA HB HC He' =>        
-        rename_i A B C;
-        let Γ' := (Hyp.val (A.subst σ) type)::Γ;
-        let Δ' := (Hyp.val A type)::Δ;
-        have S': SubstCtx σ.lift Γ' Δ'
-          := S.lift_delta (by exact HA)
-        let Γ'' := (Hyp.val (B.subst σ.lift) prop)::Γ';
-        let Δ'' := (Hyp.val B prop)::Δ';
-        have S'': SubstCtx σ.lift.lift Γ'' Δ''
-          := S'.lift_delta (by exact HB);
-        have Ie'' := 
-          loosen Ie' He' S'' 
-          (false::true::Γ.sparsity) (false::true::Δ.sparsity);
-        dsimp only [stlc, Stlc.subst, Subst.liftn]
-        conv =>
-          lhs
-          congr
-          . rw [(HasType.set HA HB).stlc_ty_subst]
-          . rw [Ie He S]
-          . rw [Ie'']
-            rw [Subst.stlc_lift_false]
-            rw [Subst.stlc_lift_true]
-      | let_repr He HA HB HC He' =>        
-        rename_i A B C;
-        let Γ' := (Hyp.gst (A.subst σ))::Γ;
-        let Δ' := (Hyp.gst A)::Δ;
-        have S': SubstCtx σ.lift Γ' Δ'
-          := S.lift_delta (by exact HA)
-        let Γ'' := (Hyp.val (B.subst σ.lift) type)::Γ';
-        let Δ'' := (Hyp.val B type)::Δ';
-        have S'': SubstCtx σ.lift.lift Γ'' Δ''
-          := S'.lift_delta (by exact HB);
-        have Ie'' := 
-          loosen Ie' He' S'' 
-          (true::false::Γ.sparsity) (true::false::Δ.sparsity);
-        have HB': ((Hyp.val A type)::Δ) ⊢ B: type
-          := by {
-            apply HB.sub;
-            constructor
-            exact Context.is_sub.refl;
-            constructor
-            constructor
-          }
-        dsimp only [stlc, Stlc.subst, Subst.liftn]
-        conv =>
-          lhs
-          congr
-          . rw [(HasType.union HA HB').stlc_ty_subst]
-          . rw [Ie He S]
-          . rw [Ie'']
-            rw [Subst.stlc_lift_true]
-            rw [Subst.stlc_lift_false]
-    case bin k l r Il Ir => 
-      cases H with
-      | pair HP Hl Hr => 
-        dsimp only [stlc, Stlc.subst]
-        conv =>
-          lhs
-          congr
-          . rw [Il Hl S]
-          . rw [Ir Hr S]
-      | elem HP Hl Hr => 
-        dsimp only [stlc, Stlc.subst]
-        rw [Il Hl S]
-      | repr HP Hl Hr => 
-        dsimp only [stlc, Stlc.subst]
-        rw [Ir Hr S]
-    -- TODO: potential bug: when A shadows A', there's an error
-    -- (2022-04-26, 23:15)
-    case abs k A' t _ It => 
-      have SA: ∀k, (Δ ⊢ A': k.annot) -> 
-        SubstCtx σ.lift ((Hyp.mk (A'.subst σ) k)::Γ) ((Hyp.mk A' k)::Δ)
-        := λk HA => S.lift_delta HA
-      cases H with
-      | lam Ht HA => 
-        dsimp only [stlc, Stlc.subst]
-        conv =>
-          lhs
-          congr
-          . rw [HA.stlc_ty_subst]
-          . rw [
-              loosen It Ht (SA _ (by exact HA)) 
-              (true::Γ.sparsity) (true::Δ.sparsity)
-              rfl rfl
-            ]
-            rhs
-            rw [Subst.stlc_lift_true]
-      | _ => 
-        rename _ ⊢ t: _ => Ht;
-        rename _ ⊢ A': _ => HA;
-        dsimp only [stlc, Stlc.subst]
-        rw [
-          loosen It Ht (SA _ (by exact HA)) 
-          (false::Γ.sparsity) (false::Δ.sparsity)
-          rfl rfl
-        ]
-        rw [Subst.stlc_lift_false]
-    case tri k X l r IX Il Ir => 
-      cases H with
-      | app HAB Hl Hr => 
-        dsimp only [stlc, Stlc.subst]
-        conv =>
-          lhs
-          congr
-          . rw [HAB.stlc_ty_subst]
-          . rw [Il Hl S]
-          . rw [Ir Hr S]
-      | app_pr HAB Hl Hr => 
-        dsimp only [stlc, Stlc.subst]
-        rw [Il Hl S]
-      | app_irrel HAB Hl Hr => 
-        dsimp only [stlc, Stlc.subst]
-        rw [Il Hl S]
-    case cases k C d l r IC Id Il Ir => 
-      cases H with
-      | case Hd HA HB HC Hl Hr => 
-        rename_i A B C;
-        have SA 
-          : SubstCtx σ.lift ((Hyp.val (A.subst σ) type)::Γ) ((Hyp.val A type)::Δ)
-          := S.lift_delta (by exact HA)
-        have SB 
-          : SubstCtx σ.lift ((Hyp.val (B.subst σ) type)::Γ) ((Hyp.val B type)::Δ)
-          := S.lift_delta (by exact HB);
-        dsimp only [stlc, Stlc.subst]
-        conv =>
-          lhs
-          congr
-          . rw [(HasType.coprod HA HB).stlc_ty_subst]
-          . rw [Id Hd S]
-          . rw [loosen Il Hl SA (true::Γ.sparsity) (true::Δ.sparsity)]
-            rhs
-            rw [Subst.stlc_lift_true]
-          . rw [loosen Ir Hr SB (true::Γ.sparsity) (true::Δ.sparsity)]
-            rhs
-            rw [Subst.stlc_lift_true]
-    case nr k K e z s _ Ie Iz Is => 
-      cases H with
-      | natrec HK He Hz Hs => 
-        let Γ' := (Hyp.gst nats)::Γ;
-        let Δ' := (Hyp.gst nats)::Δ;
-        have S': SubstCtx σ.lift Γ' Δ'
-          := S.lift_delta (by constructor)
-        let Γ'' := (Hyp.val (K.subst σ.lift) type)::Γ';
-        let Δ'' := (Hyp.val K type)::Δ';
-        -- BUG?: why is it that if the `by exact` is removed for argument 2, 
-        -- there's an error? (2022-04-25, 16:34)
-        --
-        -- Note on (2022-04-26, 23:46): same thing with `lift_delta`;
-        -- think it has to do with unification...
-        --
-        -- Note on (2022-05-13, 15:21): still have the same error...
-        have S'': SubstCtx σ.lift.lift Γ'' Δ''
-          := S'.lift_delta (by exact HK);
-        have Is'' := 
-          loosen Is Hs S'' 
-          (true::false::Γ.sparsity) (true::false::Δ.sparsity);
-        dsimp only [subst, stlc, Stlc.subst, Subst.liftn]
-        simp only [if_pos True.intro]
-        conv =>
-          lhs
-          congr
-          . rw [HK.stlc_ty_subst]
-          . rw [Ie He S]
-          . rw [Iz Hz S]
-          . rw [Is'']
-            rhs
-            rw [Subst.stlc_lift_true]
-            rw [Subst.stlc_lift_false]
-    all_goals (cases H)
-  }
+  : (a.subst σ).stlc
+  = (a.stlc).subst σ.stlc
+  := sorry
 
 abbrev SubstCtx.interp {σ Γ Δ} (S: SubstCtx σ Γ Δ) (IΔ: IsCtx Δ)
   : Stlc.InterpSubst Γ.stlc Δ.stlc
   := Stlc.SubstCtx.interp (S.stlc IΔ)
 
-theorem SubstCtx.interp_lift_ty 
-  {σ: Subst} {Γ Δ: Context} {A}
+theorem SubstCtx.interp_lift
+  {σ: Subst} {Γ Δ: Context} {A s}
   (S: SubstCtx σ Γ Δ)
   (S': 
     SubstCtx σ.lift 
-      ({ ty := A.subst σ, kind := HypKind.val type }::Γ) 
-      ({ ty := A, kind := HypKind.val type }::Δ))
+      ({ ty := A.subst σ, kind := HypKind.val s }::Γ) 
+      ({ ty := A, kind := HypKind.val s }::Δ))
   (IΔ: IsCtx Δ)
-  (HA: Δ ⊢ A: type)
+  (HA: Δ ⊢ A: sort s)
   : S'.interp (IsCtx.cons_val IΔ HA) 
   = cast (by simp only [Context.stlc]; rw [HA.stlc_ty_subst])
     (@Stlc.InterpSubst.lift A.stlc_ty Γ.stlc Δ.stlc (S.interp IΔ))
@@ -351,8 +93,9 @@ theorem SubstCtx.interp_lift_ty
           rw [<-Stlc.HasType.interp_wk1 _ x]
         apply congr _ rfl;
         apply interp_congr;
-        simp [Subst.stlc_lift_true]
-        rfl
+        simp [Subst.stlc_lift, Subst.stlc]
+        --TODO: fix this...
+        sorry
   }
 
 abbrev SubstCtx.interp_up {σ Γ Δ} (S: SubstCtx σ Γ Δ) (IΔ: IsCtx Δ)
@@ -371,15 +114,15 @@ abbrev SubstCtx.transport_interp {σ Γ Δ}
   : Δ.stlc.interp
   := Stlc.InterpSubst.transport_ctx (S.interp IΔ) G
 
-theorem SubstCtx.transport_interp_lift_ty 
-  {σ: Subst} {Γ Δ: Context} {A}
+theorem SubstCtx.transport_interp_lift
+  {σ: Subst} {Γ Δ: Context} {A s}
   (S: SubstCtx σ Γ Δ)
   (S': 
     SubstCtx σ.lift 
-      ({ ty := A.subst σ, kind := HypKind.val type }::Γ) 
-      ({ ty := A, kind := HypKind.val type }::Δ))
+      ({ ty := A.subst σ, kind := HypKind.val s }::Γ) 
+      ({ ty := A, kind := HypKind.val s }::Δ))
   (IΔ: IsCtx Δ)
-  (HA: Δ ⊢ A: type)
+  (HA: Δ ⊢ A: sort s)
   (G: Γ.stlc.interp)
   (x y)
   (p: x = HA.stlc_ty_subst ▸ y)
@@ -401,7 +144,7 @@ theorem SubstCtx.transport_interp_lift_ty
       ]
     }
     {
-      rw [interp_lift_ty S S' IΔ HA]
+      rw [interp_lift S S' IΔ HA]
       --TODO: report broken binding here...
       rw [Stlc.InterpSubst.pop_cast']
       rw [Stlc.InterpSubst.pop_lift_step]
@@ -417,41 +160,6 @@ theorem SubstCtx.transport_interp_lift_ty
       rfl
     }
   }
-  
-theorem SubstCtx.transport_interp_lift_prop
-  {σ: Subst} {Γ Δ: Context} {A}
-  (S: SubstCtx σ Γ Δ)
-  (S': 
-    SubstCtx σ.lift 
-      ({ ty := A.subst σ, kind := HypKind.val prop }::Γ) 
-      ({ ty := A, kind := HypKind.val prop }::Δ))
-  (IΔ: IsCtx Δ)
-  (HA: Δ ⊢ A: prop)
-  (G: Γ.stlc.interp)
-  : transport_interp S' (IsCtx.cons_val IΔ HA) G
-  = transport_interp S IΔ G
-  := by {
-    unfold transport_interp
-    unfold Stlc.InterpSubst.transport_ctx
-    simp only [Context.stlc]
-    apply congr _ rfl;
-    {
-      funext h;
-      generalize HI: interp S _ = I;
-      generalize HI': interp S' _ = I';
-      have HII': I = I' := by {
-        rw [<-HI];
-        rw [<-HI'];
-        unfold interp;
-        funext n A Hv G;
-        unfold Stlc.SubstCtx.interp;
-        apply congr _ rfl;
-        apply interp_congr;
-        simp [Subst.stlc_lift_false]
-      };
-      rw [HII']
-    }
-  }
 
 abbrev SubstCtx.transport_interp_up {σ Γ Δ}
   (S: SubstCtx σ Γ Δ)
@@ -460,15 +168,15 @@ abbrev SubstCtx.transport_interp_up {σ Γ Δ}
   : Δ.upgrade.stlc.interp
   := transport_interp S.upgrade IΔ.upgrade G
 
-theorem SubstCtx.transport_interp_up_lift_ty 
-  {σ: Subst} {Γ Δ: Context} {A}
+theorem SubstCtx.transport_interp_up_lift
+  {σ: Subst} {Γ Δ: Context} {A s}
   (S: SubstCtx σ Γ Δ)
   (S': 
     SubstCtx σ.lift 
-      ({ ty := A.subst σ, kind := HypKind.val type }::Γ) 
-      ({ ty := A, kind := HypKind.val type }::Δ))
+      ({ ty := A.subst σ, kind := HypKind.val s }::Γ) 
+      ({ ty := A, kind := HypKind.val s }::Δ))
   (IΔ: IsCtx Δ)
-  (HA: Δ ⊢ A: type)
+  (HA: Δ ⊢ A: sort s)
   (G: Γ.upgrade.stlc.interp)
   (x y)
   (p: x = HA.stlc_ty_subst ▸ y)
@@ -476,137 +184,75 @@ theorem SubstCtx.transport_interp_up_lift_ty
   = (x, transport_interp_up S IΔ G)
   := by {
     unfold transport_interp_up
-    apply transport_interp_lift_ty;
+    apply transport_interp_lift;
     exact p;
-    exact HA.upgrade
-  }
-  
-theorem SubstCtx.transport_interp_up_lift_prop
-  {σ: Subst} {Γ Δ: Context} {A}
-  (S: SubstCtx σ Γ Δ)
-  (S': 
-    SubstCtx σ.lift 
-      ({ ty := A.subst σ, kind := HypKind.val prop }::Γ) 
-      ({ ty := A, kind := HypKind.val prop }::Δ))
-  (IΔ: IsCtx Δ)
-  (HA: Δ ⊢ A: prop)
-  (G: Γ.upgrade.stlc.interp)
-  : transport_interp_up S' (IsCtx.cons_val IΔ HA) G
-  = transport_interp_up S IΔ G
-  := by {
-    unfold transport_interp_up
-    apply transport_interp_lift_prop;
     exact HA.upgrade
   }
 
 theorem HasType.subst_stlc_interp_commute {Γ Δ σ a} 
-  (H: Δ ⊢ a: expr s A) 
+  (H: Δ ⊢ a: term A) 
   (S: SubstCtx σ Γ Δ)
   (IΔ: IsCtx Δ)
   (G: Γ.stlc.interp)
   : (H.subst S).stlc.interp G
   = (Annot.stlc_ty_subst H.expr_regular) ▸ H.stlc.interp.subst (S.interp IΔ) G
   := by {
-    cases s with
-    | type =>
-      rw [<-Stlc.HasType.subst_interp_dist]
-      rw [rec_to_cast']
-      rw [Stlc.HasType.interp_transport_cast']
-      rw [Term.term_subst_stlc_commute]
-      assumption
-      assumption
-      rw [Annot.stlc_ty_subst H.expr_regular]
-    | prop => 
-      generalize Stlc.HasType.interp _ _ = x;
-      generalize Stlc.Context.deriv.subst _ _ _ = y;
-      cases x with
-      | none => 
-        cases y with
-        | none => simp
-        | some x => cases x
-      | some x => cases x
+    rw [<-Stlc.HasType.subst_interp_dist]
+    rw [rec_to_cast']
+    rw [Stlc.HasType.interp_transport_cast']
+    rw [Term.term_subst_stlc_commute]
+    assumption
+    assumption
+    rw [Annot.stlc_ty_subst H.expr_regular]
   }
   
 theorem HasType.subst_stlc_interp_up_commute {Γ Δ σ a} 
-  (H: Δ.upgrade ⊢ a: expr s A) 
+  (H: Δ.upgrade ⊢ a: term A) 
   (S: SubstCtx σ Γ Δ)
   (IΔ: IsCtx Δ)
   (G: Γ.upgrade.stlc.interp)
   : (H.subst S.upgrade).stlc.interp G
   = (Annot.stlc_ty_subst H.expr_regular) ▸ H.stlc.interp.subst (S.interp_up IΔ) G
   := by {
-    cases s with
-    | type =>
-      rw [<-Stlc.HasType.subst_interp_dist]
-      rw [rec_to_cast']
-      rw [Stlc.HasType.interp_transport_cast']
-      rw [Term.term_subst_stlc_commute]
-      assumption
-      apply SubstCtx.upgrade S;
-      rw [Annot.stlc_ty_subst H.expr_regular]
-    | prop =>
-      generalize Stlc.HasType.interp _ _ = x;
-      generalize Stlc.Context.deriv.subst _ _ _ = y;
-      cases x with
-      | none => 
-        cases y with
-        | none => simp
-        | some x => cases x
-      | some x => cases x
+    rw [<-Stlc.HasType.subst_interp_dist]
+    rw [rec_to_cast']
+    rw [Stlc.HasType.interp_transport_cast']
+    rw [Term.term_subst_stlc_commute]
+    assumption
+    apply SubstCtx.upgrade S;
+    rw [Annot.stlc_ty_subst H.expr_regular]
   }
 
 theorem HasType.subst_stlc_interp_commute' {Γ Δ σ a} 
-  (H: Δ ⊢ a: expr s A) 
+  (H: Δ ⊢ a: term A) 
   (S: SubstCtx σ Γ Δ)
   (IΔ: IsCtx Δ)
   (G: Γ.stlc.interp)
   : (Annot.stlc_ty_subst H.expr_regular) ▸ (H.subst S).stlc.interp G
   = H.stlc.interp.subst (S.interp IΔ) G
   := by {
-    cases s with
-    | type =>
-      rw [<-Stlc.HasType.subst_interp_dist]
-      rw [rec_to_cast']
-      rw [Stlc.HasType.interp_transport_cast']
-      rw [Term.term_subst_stlc_commute]
-      assumption
-      assumption
-      rw [Annot.stlc_ty_subst H.expr_regular]
-    | prop =>
-      generalize Stlc.HasType.interp _ _ = x;
-      generalize Stlc.Context.deriv.subst _ _ _ = y;
-      cases x with
-      | none => 
-        cases y with
-        | none => simp
-        | some x => cases x
-      | some x => cases x
+    rw [<-Stlc.HasType.subst_interp_dist]
+    rw [rec_to_cast']
+    rw [Stlc.HasType.interp_transport_cast']
+    rw [Term.term_subst_stlc_commute]
+    assumption
+    assumption
+    rw [Annot.stlc_ty_subst H.expr_regular]
   }
   
 theorem HasType.subst_stlc_interp_up_commute' {Γ Δ σ a} 
-  (H: Δ.upgrade ⊢ a: expr s A) 
+  (H: Δ.upgrade ⊢ a: term A) 
   (S: SubstCtx σ Γ Δ)
   (IΔ: IsCtx Δ)
   (G: Γ.upgrade.stlc.interp)
   : (Annot.stlc_ty_subst H.expr_regular) ▸ (H.subst S.upgrade).stlc.interp G
   = H.stlc.interp.subst (S.interp_up IΔ) G
   := by {
-    cases s with
-    | type =>
-      rw [<-Stlc.HasType.subst_interp_dist]
-      rw [rec_to_cast']
-      rw [Stlc.HasType.interp_transport_cast']
-      rw [Term.term_subst_stlc_commute]
-      assumption
-      apply SubstCtx.upgrade S;
-      rw [Annot.stlc_ty_subst H.expr_regular]
-    | prop =>
-      generalize Stlc.HasType.interp _ _ = x;
-      generalize Stlc.Context.deriv.subst _ _ _ = y;
-      cases x with
-      | none => 
-        cases y with
-        | none => simp
-        | some x => cases x
-      | some x => cases x
+    rw [<-Stlc.HasType.subst_interp_dist]
+    rw [rec_to_cast']
+    rw [Stlc.HasType.interp_transport_cast']
+    rw [Term.term_subst_stlc_commute]
+    assumption
+    apply SubstCtx.upgrade S;
+    rw [Annot.stlc_ty_subst H.expr_regular]
   }
