LogicalRefinement/Stlc/InterpWk.lean
@@ -2,22 +2,19 @@ import LogicalRefinement.Untyped
 import LogicalRefinement.Typed
 import LogicalRefinement.Stlc.Basic
 import LogicalRefinement.Stlc.Interp
-import LogicalRefinement.Stlc.InterpWkUtils
 import LogicalRefinement.Stlc.InterpSubst
-import LogicalRefinement.Stlc.InterpInv
 import LogicalRefinement.Stlc.Subst
 open Annot
 open AnnotSort
 
-def Wk.stlc (ρ: Wk) (Γ: Sparsity) (Δ: Sparsity): Stlc.Subst 
-  := ρ.to_subst.stlc Γ Δ
-
 theorem Term.wk_stlc_commute {Γ Δ ρ a} 
   (H: Δ ⊢ a: term A) 
   (R: WkCtx ρ Γ Δ)
-  : (a.wk ρ).stlc Γ.sparsity
-  = (a.stlc Δ.sparsity).subst (ρ.stlc Γ.sparsity Δ.sparsity)
+  : (a.wk ρ).stlc
+  = a.stlc.wk ρ
   := by {
     rw [<-Subst.subst_wk_compat]
-    apply Term.term_subst_stlc_commute H R.to_subst
+    --TODO: this rw [<-Stlc.Subst.subst_wk_compat]
+    --apply Term.term_subst_stlc_commute H R.to_subst
+    sorry
   }
