LogicalRefinement/Stlc.lean
@@ -1,9 +1,7 @@
 prelude
 import LogicalRefinement.Stlc.Basic
 import LogicalRefinement.Stlc.Interp
-import LogicalRefinement.Stlc.InterpInv
 import LogicalRefinement.Stlc.InterpSubst
-import LogicalRefinement.Stlc.InterpWkUtils
 import LogicalRefinement.Stlc.InterpWk
 import LogicalRefinement.Stlc.InterpUpgrade
 import LogicalRefinement.Stlc.Subst
