LogicalRefinement/Stlc/InterpUpgrade.lean
@@ -2,8 +2,6 @@ import LogicalRefinement.Untyped
 import LogicalRefinement.Typed
 import LogicalRefinement.Stlc.Basic
 import LogicalRefinement.Stlc.Interp
-import LogicalRefinement.Stlc.InterpWkUtils
-import LogicalRefinement.Stlc.InterpInv
 import LogicalRefinement.Stlc.Subst
 import LogicalRefinement.Stlc.InterpSubst
 import LogicalRefinement.Stlc.InterpWk
