LogicalRefinement/Stlc/Utils.lean
@@ -2,7 +2,6 @@ import LogicalRefinement.Untyped
 import LogicalRefinement.Typed
 import LogicalRefinement.Stlc.Basic
 import LogicalRefinement.Stlc.Interp
-import LogicalRefinement.Stlc.InterpInv
 import LogicalRefinement.Stlc.InterpSubst
 import LogicalRefinement.Stlc.InterpWk
 import LogicalRefinement.Stlc.Subst
@@ -10,100 +9,21 @@ import LogicalRefinement.Stlc.Subst
 open Annot
 open AnnotSort
 
-theorem HasVar.stlc_var {Γ n A} (H: HasVar Γ n (HypKind.val type) A)
-  : (Term.var n).stlc Γ.sparsity = Stlc.var (Γ.sparsity.ix n)
-  := by {
-    dsimp only [Term.stlc, Sparsity.stlc]
-    rw [if_pos]
-    rw [H.sigma]
-    rfl
-  }
+theorem HasVar.stlc_var {Γ n A} (_: HasVar Γ n (HypKind.val type) A)
+  : (Term.var n).stlc = Stlc.var n
+  := rfl
 
 theorem HasType.stlc_var_term {Γ n A} (H: Γ ⊢ Term.var n: term A)
-  : (Term.var n).stlc Γ.sparsity = Stlc.var (Γ.sparsity.ix n)
+  : (Term.var n).stlc = Stlc.var n
   := HasVar.stlc_var (by cases H <;> assumption)
 
 theorem HasType.stlc_interp_var {Γ n A} (H: Γ ⊢ Term.var n: term A):
   H.stlc.interp = H.to_var.stlc.interp
   := by {
-    dsimp only [Context.stlc_ix]
     funext G;
     rw [<-
       Stlc.HasType.interp_transport_inner (Stlc.HasType.var H.to_var.stlc) 
       _ H.stlc_var_term.symm rfl
     ]
-    rfl
-  }
-
-theorem Stlc.Context.thin_upgrade {Γ: _root_.Context}:
-    Γ.upgrade.stlc.thin Γ.upgrade.downgrade_sparsity =
-    Γ.upgrade.stlc
-    := by {
-      induction Γ with
-      | nil => rfl
-      | cons H Γ I =>
-        cases H with
-        | mk A k =>
-          cases k with
-          | val s => 
-            cases s with
-            | type => exact congr rfl I
-            | prop => exact I
-          | gst => exact congr rfl I
-    }
-  
-theorem Stlc.Context.thin_double_upgrade_helper {Γ: _root_.Context}:
-    Γ.upgrade.upgrade.stlc.thin Γ.upgrade.downgrade_sparsity =
-    Γ.upgrade.upgrade.stlc
-    := by {
-      rw [Context.upgrade_idem]
-      exact thin_upgrade
-    }
-
-theorem Stlc.Context.thin_upgrade_cast
-  {Γ: _root_.Context} (G: Γ.upgrade.upgrade.stlc.interp)
-  : G.thin Γ.upgrade.downgrade_sparsity
-  = cast (by rw [thin_double_upgrade_helper]) G
-  := by {
-    induction Γ with
-    | nil => rfl
-    | cons H Γ I => 
-      cases H with
-      | mk A k => 
-        cases k with
-        | val s =>
-          cases s with
-          | type =>
-            cases G with
-            | mk x G => 
-              simp only [interp.thin, Context.downgrade_sparsity]
-              rw [cast_pair']
-              apply congr rfl;
-              exact I G
-              rfl
-          | prop => 
-              simp only [interp.thin, Context.downgrade_sparsity]
-              exact I G
-        | gst => 
-          cases G with
-          | mk x G => 
-            simp only [interp.thin, Context.downgrade_sparsity]
-            rw [cast_pair']
-            apply congr rfl;
-            exact I G
-            rfl
-  }
-
-theorem Stlc.Context.interp.downgrade_cast
-  {Γ: _root_.Context} (G: Γ.upgrade.stlc.interp)
-  (p: Γ.upgrade.stlc.interp = Γ.upgrade.upgrade.stlc.interp)
-  : (cast p G).downgrade = G
-  := by {
-    unfold downgrade
-    unfold Eq.mpr
-    rw [rec_to_cast']
-    rw [thin_upgrade_cast]
-    rw [cast_merge]
-    rw [cast_merge]
     rfl
   }
